Hs/Metatheory/WeakenCompile.lean
@@ -6,34 +6,282 @@ import Hs.Metatheory.Uniqueness
 
 set_option maxHeartbeats 1000000
 
-theorem weaken_compile_kind f :
-  (j : Γ ⊢κ t : k) ->
-  (sj : (f :: Γ) ⊢κ ([S]t) : ([S]k)) ->
-  compile_kind Γ t k j = .some t' ->
-  compile_kind (f::Γ) ([S]t) ([S]k) sj = .some ([S]t') := by
-intro j sj c;
-induction Γ, t, k, j using compile_kind.induct generalizing t';
-case _ =>
-  unfold compile_kind; cases sj; simp; unfold compile_kind at c; cases c; simp;
-case _ j1 j2 ih1 ih2 =>
-  unfold compile_kind at c; simp at c;
-  rw[Option.bind_eq_some] at c;
-  cases c; case _ wa c =>
-  cases c; case _ ca cb =>
-  rw[Option.bind_eq_some] at cb;
-  cases cb; case _ wb cb =>
-  cases cb; case _ cb e =>
-  cases e; cases sj;
-  case _ jaw jbw =>
-  have ih1' := @ih1 wa jaw ca
-  have ih2' := @ih2 wb jbw cb
-  unfold compile_kind; simp;
-  rw[Option.bind_eq_some];
-  exists ([S]wa); apply And.intro;
-  assumption;
-  rw[Option.bind_eq_some];
-  exists ([S]wb);
+theorem compile_kind_congr :
+  (∀ (Γ : Ctx HsTerm) (h1 h2 : ⊢s Γ), h1 = h2) ->
+  B = B' -> k = k' ->
+  (sj : Γ ⊢κ B : k) -> (sj' : Γ ⊢κ B' : k') ->
+  compile_kind Γ B k sj = compile_kind Γ B' k' sj' := by
+intro h e1 e2 sj sj';
+subst e1; subst e2;
+have u := kinds_have_unique_judgments h sj sj';
+subst u; simp;
 
+theorem rename_compile_kind (r : Ren) : (t k : HsTerm) -> (t' : Term) ->
+  (∀ (Γ : Ctx HsTerm) (h1 h2 : ⊢s Γ), h1 = h2) ->
+  (j : Γ ⊢κ t : k) ->
+  compile_kind Γ t k j = .some t' ->
+  (wf : ⊢s Δ) ->
+  (rctx : ∀ x, (Γ d@ x).apply r.to = Δ d@ (r x)) ->
+  (sj : Δ ⊢κ ([r.to]t) : ([r.to]k)) ->
+  compile_kind Δ ([r.to]t) ([r.to]k) sj = .some ([r.to]t') := by
+intro t k t' h1 j ck wf h2 sj;
+induction Γ, t, k, j using compile_kind.induct generalizing Δ t' <;> simp
+case _ =>
+  unfold compile_kind at ck; cases ck
+  cases sj; simp;
+  unfold compile_kind; rfl
+case _ Γ A B j1 j2 ih1 ih2 =>
+  unfold compile_kind at ck; simp at ck;
+  rw[Option.bind_eq_some] at ck;
+  cases ck; case _ A' ck =>
+  cases ck; case _ cA ck =>
+  rw[Option.bind_eq_some] at ck;
+  cases ck; case _ B' ck =>
+  cases ck; case _ cB ck =>
+  cases ck
+  simp at sj; cases sj; case _ jA' jB' =>
+  unfold compile_kind; simp
+  have ih1' := @ih1 Δ A' cA wf h2 jA'
+  have ih2' := @ih2 Δ B' cB wf h2 jB'
+  cases sj; simp;
+  rw[Option.bind_eq_some]; exists ([r.to]A')
+  constructor;
+  case _ =>
+    rw[<-ih1']
+    apply compile_kind_congr h1
+    unfold Subst.apply; simp
+    simp
+  rw[Option.bind_eq_some]; exists ([r.to]B')
+  constructor;
+  case _ =>
+    rw[<-ih2']
+    apply compile_kind_congr h1
+    unfold Subst.apply; simp
+    simp
+  simp
+
+
+theorem weaken_compile_kind f :
+  (∀ (Γ : Ctx HsTerm) (h1 h2 : ⊢s Γ), h1 = h2) ->
+  (j : Γ ⊢κ t : k) ->
+  compile_kind Γ t k j = .some t' ->
+  Γ ⊢s f ->
+  (sj : (f :: Γ) ⊢κ ([S]t) : ([S]k)) ->
+  compile_kind (f::Γ) ([S]t) ([S]k) sj = .some ([S]t') := by
+intro wfeq j c h;
+apply rename_compile_kind (λ x => (x + 1)) _ _ _ wfeq j c;
+case _ => apply hs_frame_wf_implies_wkn_wf h
+case _ =>
+  intro x; simp;
+  generalize fh : Γ d@ x = f at *;
+  cases f
+  all_goals try (unfold Frame.apply; simp; congr)
+  unfold Frame.apply; simp
+  all_goals(constructor; unfold S; congr; unfold S; congr)
+
+theorem compile_type_congr :
+  (∀ (Γ : Ctx HsTerm) (h1 h2 : ⊢s Γ), h1 = h2) ->
+  B = B' -> k = k' ->
+  (sj : Γ ⊢τ B : k) -> (sj' : Γ ⊢τ B' : k') ->
+  compile_type Γ B k sj = compile_type Γ B' k' sj' := by
+intro h e1 e2 sj sj';
+subst e1; subst e2;
+have u := types_have_unique_judgments h sj sj';
+subst u; simp;
+
+theorem rename_compile_type (r : Ren) : (t k : HsTerm) -> (t' : Term) ->
+  (∀ (Γ : Ctx HsTerm) (h1 h2 : ⊢s Γ), h1 = h2) ->
+  (j : Γ ⊢τ t : k) ->
+  compile_type Γ t k j = .some t' ->
+  (wf : ⊢s Δ) ->
+  (rctx : ∀ x, (Γ d@ x).apply r.to = Δ d@ (r x)) ->
+  (sj : Δ ⊢τ ([r.to]t) : ([r.to]k)) ->
+  compile_type Δ ([r.to]t) ([r.to]k) sj = .some ([r.to]t') := by
+intro t k t' h1 j cj wf h2 sj -- sjR;
+induction Γ, t, k, j using compile_type.induct generalizing Δ t' r
+all_goals (unfold compile_type at cj; simp at cj)
+case _ Γ T x wf' c gt jk  =>
+  have j : Γ ⊢τ `#x : T := by constructor; assumption; assumption; assumption; assumption
+  rw[Option.bind_eq_some] at cj;
+  cases cj; case _ T' cj =>
+  cases cj; case _ cT cj =>
+  cases cj;
+  unfold compile_type; simp;
+  have sj' := @hs_rename Γ Δ r .type (`#x, T) j wf h2
+  have u := types_have_unique_judgments h1 sj' sj
+  subst u; cases sj'; case _ wf c' jk' gt' =>
+  simp;
+  rw[Option.bind_eq_some];
+  exists ([r.to]T')
+  constructor;
+  case _ =>
+    apply @rename_compile_kind Γ Δ r T `□
+    assumption
+    assumption
+    assumption
+    assumption
+  simp; unfold Ren.to; simp;
+case _ Γ B f A a j1 j2 j3 j4 ih1 ih2 =>
+  rw[Option.bind_eq_some] at cj;
+  cases cj; case _ A' cj =>
+  cases cj; case _ cA cj =>
+  rw[Option.bind_eq_some] at cj;
+  cases cj; case _ B' cj =>
+  cases cj; case _ cB cj =>
+  rw[Option.bind_eq_some] at cj;
+  cases cj; case _ f' cj =>
+  cases cj; case _ cf cj =>
+  rw[Option.bind_eq_some] at cj;
+  cases cj; case _ a' cj =>
+  cases cj; case _ ca cj =>
+  cases cj;
+  cases sj; case _ α jka ja' jbk jb' =>
+  unfold compile_type; simp;
+  have j2' := @hs_rename Γ Δ r .type (a, A) j2 wf h2; simp at j2';
+  have j1' := @hs_rename Γ Δ r .type (f, (A `-k> B)) j1 wf h2; simp at j1'
+  have u1 := kinds_subst_eff_free_types (r.to) (A `-k> B) j1; simp at u1;
+  have ua := idempotent_substitution_typing r.to A j2;
+  have u := types_have_unique_judgments h1 ja'
+  have ih1' := @ih1 Δ r f' cf wf h2 j1'
+  have ih2' := @ih2 Δ r a' ca wf h2 j2'
+  have uα : α = [r.to]A := by
+    unfold Subst.apply at j2';
+    have u := types_have_unique_kinds ja' j2';
+    rw[u]; simp; unfold Subst.apply; simp;
+  rw[Option.bind_eq_some]; exists ([r.to]A')
+  constructor;
+  case _ =>
+    subst uα;
+    apply @rename_compile_kind Γ Δ r A `□;
+    assumption
+    assumption
+    assumption
+    assumption
+  rw[Option.bind_eq_some]; exists ([r.to]B')
+  constructor;
+  case _ =>
+    apply @rename_compile_kind Γ Δ r B `□;
+    assumption
+    assumption
+    assumption
+    assumption
+  rw[Option.bind_eq_some]; exists ([r.to]f')
+  constructor;
+  case _ =>
+    rw[<-ih1']
+    apply compile_type_congr h1
+    unfold Subst.apply; simp
+    simp; assumption
+  rw[Option.bind_eq_some]; exists ([r.to]a')
+  constructor;
+  case _ =>
+    rw[<-ih2']
+    apply compile_type_congr h1
+    unfold Subst.apply; simp
+    assumption
+  simp
+
+case _ Γ A B j1 j2 ih =>
+  rw[Option.bind_eq_some] at cj;
+  cases cj; case _ A' cj =>
+  cases cj; case _ cA cj =>
+  rw[Option.bind_eq_some] at cj;
+  cases cj; case _ B' cj =>
+  cases cj; case _ cB cj =>
+  cases cj;
+  cases sj; case _ sjA sjB =>
+  simp;
+  have sjB' := sjB;
+  rw[<-@HsTerm.subst_const r.lift.to] at sjB'
+  rw[<-Subst.lift_lemma] at sjB';
+  have wf' : ⊢s (.kind ([r.to]A) :: Δ) := by constructor; assumption; assumption
+  have h2' := hs_rename_lift r (.kind A) h2
+  have h3 := @rename_compile_kind Γ Δ r A `□ A' h1 j1 cA wf h2 sjA
+  have ih := @ih (.kind ([r.to]A) :: Δ) (Ren.lift r) B' cB wf' h2' sjB'
+  unfold compile_type; simp;
+  rw[Option.bind_eq_some]
+  exists ([r.to] A')
+  constructor; assumption
+  rw[Option.bind_eq_some]
+  exists ([^r.to] B')
+  constructor;
+  have e : `★ = [r.lift.to] `★ := by simp
+  have u1 : [r.lift.to]B' = [^r.to]B' := by congr; rw[Subst.lift_lemma]
+  rw[u1] at ih; rw[<-ih];
+  apply compile_type_congr h1;
+  have u2 : HsTerm.smap Subst.lift (^r.to) B = [r.lift.to]B := by
+    rw[Subst.lift_lemma]; unfold Subst.apply; simp
+  apply u2
+  apply e
+  simp
+
+case _ Γ A B j1 j2 ih1 ih2 =>
+  rw[Option.bind_eq_some] at cj;
+  cases cj; case _ A' cj =>
+  cases cj; case _ cA cj =>
+  rw[Option.bind_eq_some] at cj;
+  cases cj; case _ B' cj =>
+  cases cj; case _ cB cj =>
+  cases cj;
+  cases sj; case _ sjA sjB =>
+  simp;
+  have sjB' := sjB;
+  rw[<-@HsTerm.subst_const r.lift.to] at sjB'
+  rw[<-Subst.lift_lemma] at sjB';
+  have wf' : ⊢s (.empty :: Δ) := by constructor; assumption
+  have h2' := hs_rename_lift r .empty h2
+  have ih1' := @ih1 Δ r A' cA wf h2 sjA
+  have ih2' := @ih2 (.empty :: Δ) (Ren.lift r) B' cB wf' h2' sjB'
+  unfold compile_type; simp;
+  rw[Option.bind_eq_some]
+  exists ([r.to] A')
+  constructor; assumption
+  rw[Option.bind_eq_some]
+  exists ([^r.to] B')
+  constructor;
+  have e : `★ = [r.lift.to] `★ := by simp
+  have u1 : [r.lift.to]B' = [^r.to]B' := by congr; rw[Subst.lift_lemma]
+  rw[u1] at ih2'; rw[<-ih2'];
+  apply compile_type_congr h1;
+  have u2 : HsTerm.smap Subst.lift (^r.to) B = [r.lift.to]B := by
+    rw[Subst.lift_lemma]; unfold Subst.apply; simp
+  apply u2
+  apply e
+  simp
+
+case _ Γ A B j1 vhv j2 ih1 ih2 =>
+  rw[Option.bind_eq_some] at cj;
+  cases cj; case _ A' cj =>
+  cases cj; case _ cA cj =>
+  rw[Option.bind_eq_some] at cj;
+  cases cj; case _ B' cj =>
+  cases cj; case _ cB cj =>
+  cases cj;
+  cases sj; case _ sjA vhv' sjB =>
+  simp;
+  have sjB' := sjB;
+  rw[<-@HsTerm.subst_const r.lift.to] at sjB'
+  rw[<-Subst.lift_lemma] at sjB';
+  have wf' : ⊢s (.empty :: Δ) := by constructor; assumption
+  have h2' := hs_rename_lift r .empty h2
+  have ih1' := @ih1 Δ r A' cA wf h2 sjA
+  have ih2' := @ih2 (.empty :: Δ) (Ren.lift r) B' cB wf' h2' sjB'
+  unfold compile_type; simp;
+  rw[Option.bind_eq_some]
+  exists ([r.to] A')
+  constructor; assumption
+  rw[Option.bind_eq_some]
+  exists ([^r.to] B')
+  constructor;
+  have e : `★ = [r.lift.to] `★ := by simp
+  have u1 : [r.lift.to]B' = [^r.to]B' := by congr; rw[Subst.lift_lemma]
+  rw[u1] at ih2'; rw[<-ih2'];
+  apply compile_type_congr h1;
+  have u2 : HsTerm.smap Subst.lift (^r.to) B = [r.lift.to]B := by
+    rw[Subst.lift_lemma]; unfold Subst.apply; simp
+  apply u2
+  apply e
+  simp
 
 theorem weaken_compile_type :
   (∀ (Γ : Ctx HsTerm) (h1 h2 : ⊢s Γ), h1 = h2) ->
@@ -43,105 +291,12 @@ theorem weaken_compile_type :
   (sj : (f :: Γ) ⊢τ ([S]t) : ([S]k)) ->
   compile_type (f :: Γ) ([S]t) ([S]k) sj = .some ([S]t') := by
 intro wfeq j c h sj;
-induction Γ, t, k, j using compile_type.induct generalizing f t' <;> simp at *;
+apply rename_compile_type (λ x => (x + 1)) _ _ _ wfeq j c;
+case _ => apply hs_frame_wf_implies_wkn_wf h
 case _ =>
-  unfold compile_type; cases sj; simp;
-  unfold compile_type at c; simp at c;
-  rw[Option.bind_eq_some] at c;
-  cases c; case _ wa c =>
-  cases c; case _ ca cb =>
-  cases cb; simp
-  rw[Option.bind_eq_some];
-  exists ([S]wa); simp;
-  case _ j _ _ sj _ =>
-    apply weaken_compile_kind f j sj ca;
-case _ Γ B fa A a j1 j2 j3 j4 ih1 ih2 =>
-  unfold compile_type at c; simp at c
-  rw[Option.bind_eq_some] at c;
-  cases c; case _ wA c =>
-  cases c; case _ cA cb =>
-  rw[Option.bind_eq_some] at cb;
-  cases cb; case _ wB cb =>
-  cases cb; case _ cB cf =>
-  rw[Option.bind_eq_some] at cf;
-  cases cf; case _ wf cf =>
-  cases cf; case _ cf ca =>
-  rw[Option.bind_eq_some] at ca;
-  cases ca; case _ wa ca =>
-  cases ca; case _ ca e =>
-  cases e;
-  have wf' := Ctx.hs_weaken_frame (hs_judgment_ctx_wf .kind j3) h
-  have lem1 : (f :: Γ) ⊢τ ([S]fa) : ([S](A `-k> B)) := by
-    apply hs_weaken_type;
-    assumption
-    assumption
-
-  unfold compile_type; cases sj; simp;
-  rw[Option.bind_eq_some]; case _ A' jA' ja' jB' jb' =>
-  have sj3 := hs_weaken_kind wf' j3
-  have sj2 := hs_weaken_type wf' j2
-  have u := types_have_unique_kinds ja' sj2; cases u
-  have u := types_have_unique_judgments wfeq lem1 jb'; cases u
-  exists ([S]wA);
-  constructor
-  case _ => apply weaken_compile_kind f j3 jA' cA
-  rw[Option.bind_eq_some]; exists ([S]wB)
-  constructor
-  case _ => apply weaken_compile_kind f j4 jB' cB
-  rw[Option.bind_eq_some]; exists ([S]wf)
-  constructor
-  case _ =>
-    have ih1' := ih1 cf h lem1
-    assumption
-  rw[Option.bind_eq_some]; exists ([S]wa)
-  constructor
-  case _ =>
-    have ih2' := ih2 ca h ja'
-    assumption
-  rfl
-
-case _ Γ A B j1 j2 ih =>
-  unfold compile_type at c; simp at c
-  rw[Option.bind_eq_some] at c;
-  cases c; case _ wA c =>
-  cases c; case _ cA cb =>
-  rw[Option.bind_eq_some] at cb;
-  cases cb; case _ wB cb =>
-  cases cb; case _ cB cf =>
-  cases cf;
-  cases sj; case _ j1' j2' =>
-
-  unfold compile_type; simp;
-  rw[Option.bind_eq_some]; exists ([S]wA)
-  constructor;
-  case _ => apply weaken_compile_kind f j1 j1' cA;
-  rw[Option.bind_eq_some]; exists ([^S]wB)
-  constructor;
-  case _ =>
-    have ih' := @ih wB f cB
-    sorry
-  simp;
-case _ j1 j2 ih1 ih2 =>
-  unfold compile_type at c; simp at c;
-  rw[Option.bind_eq_some] at c;
-  cases c; case _ wa c =>
-  cases c; case _ ca cb =>
-  rw[Option.bind_eq_some] at cb;
-  cases cb; case _ wb cb =>
-  cases cb; case _ cb e =>
-  cases e;
-  cases sj; case _ ja jb =>
-  unfold compile_type; simp;
-
-  rw[Option.bind_eq_some];
-  exists ([S]wa);
-  constructor
-  case _ ja =>
-    sorry
-  rw[Option.bind_eq_some];
-  exists ([^S]wb)
-  constructor
-  sorry
-  simp
-
-case _ => sorry
+  intro x; simp;
+  generalize fh : Γ d@ x = f at *;
+  cases f
+  all_goals try (unfold Frame.apply; simp; congr)
+  unfold Frame.apply; simp
+  all_goals(constructor; unfold S; congr; unfold S; congr)
